revm: simulate: more completions

RocqOfRust/revm/revm_interpreter/instructions/simulate/macros.v
@@ -63,7 +63,7 @@ Ltac gas_macro_eq InterpreterTypesEq :=
   try (eapply Run.Call; [
     apply Run.Pure
   |]);
-  eapply Run.Call; [
+  c; [
     apply Impl_Gas.record_cost_eq
   |];
   destruct Impl_Gas.record_cost;
@@ -115,21 +115,14 @@ Definition popn_macro {WIRE K : Set} `{Link WIRE}
 
 Ltac popn_macro_eq InterpreterTypesEq :=
   unfold popn_macro;
-  eapply Run.Call; [
+  s; [
     apply InterpreterTypesEq
-      .(InterpreterTypes.Eq.StackTrait_for_Stack)
-      .(StackTrait.Eq.popn)
   |];
-  destruct _.(InterpreterTypes.StackTrait_for_Stack).(StackTrait.popn) as [[|] ?]; cbn; [|
-    apply Run.LetUnfold;
-    cbn;
-    eapply Run.Call; [
+  destruct _.(InterpreterTypes.StackTrait_for_Stack).(StackTrait.popn) as [[|] ?]; [|
+    s; [
       apply InterpreterTypesEq
-        .(InterpreterTypes.Eq.LoopControl_for_Control)
-        .(LoopControl.Eq.set_instruction_result)
     |];
-    cbn;
-    apply Run.Pure
+    s
   ].
 
 Definition popn_top_macro {WIRE K : Set} `{Link WIRE}
@@ -169,23 +162,50 @@ Definition popn_top_macro {WIRE K : Set} `{Link WIRE}
 
 Ltac popn_top_macro_eq InterpreterTypesEq :=
   unfold popn_top_macro;
-  eapply Run.Call; [
-    apply Run.Pure
-  |];
-  eapply Run.Call; [
+  s; [
     apply InterpreterTypesEq
       .(InterpreterTypes.Eq.StackTrait_for_Stack)
       .(StackTrait.Eq.popn_top)
   |];
   destruct _.(InterpreterTypes.StackTrait_for_Stack).(StackTrait.popn_top) as [[[? ?]|] ?];
   [|
-    apply Run.LetUnfold;
-    eapply Run.Call; [
+    s; [
       apply InterpreterTypesEq
         .(InterpreterTypes.Eq.LoopControl_for_Control)
         .(LoopControl.Eq.set_instruction_result)
     |];
-    apply Run.Pure
+    s
+  ].
+
+Definition push_macro {WIRE K : Set} `{Link WIRE}
+    {WIRE_types : InterpreterTypes.Types.t} `{InterpreterTypes.Types.AreLinks WIRE_types}
+    {IInterpreterTypes : InterpreterTypes.C WIRE_types}
+    (interpreter : Interpreter.t WIRE WIRE_types)
+    (value : aliases.U256.t)
+    (k_exit : Interpreter.t WIRE WIRE_types -> K)
+    (k : Interpreter.t WIRE WIRE_types -> K) :
+    K :=
+  let '(success, stack) :=
+    IInterpreterTypes.(InterpreterTypes.StackTrait_for_Stack).(StackTrait.push)
+      interpreter.(Interpreter.stack) value in
+  let interpreter := interpreter <| Interpreter.stack := stack |> in
+  if success then k interpreter
+  else
+    let control :=
+      IInterpreterTypes.(InterpreterTypes.LoopControl_for_Control).(LoopControl.set_instruction_result)
+        interpreter.(Interpreter.control)
+        instruction_result.InstructionResult.StackOverflow in
+    let interpreter := interpreter <| Interpreter.control := control |> in
+    k_exit interpreter.
+
+Ltac push_macro_eq InterpreterTypesEq :=
+  unfold push_macro;
+  s; [
+    apply InterpreterTypesEq
+  |];
+  destruct _.(InterpreterTypes.StackTrait_for_Stack).(StackTrait.push) as [[] ?]; [|
+    s; [apply InterpreterTypesEq|];
+    s
   ].
 
 Definition check_macro {WIRE K : Set} `{Link WIRE}
@@ -252,10 +272,43 @@ Ltac check_macro_eq InterpreterTypesEq :=
   ].
 
 Definition as_u64_saturated_macro (v : aliases.U256.t) : u64 :=
-  Z.min v.(Uint.value) (2 ^ 64 - 1).
+  let v0 := v.(Uint.value) mod 2^64 in
+  let v1 := (v.(Uint.value) / 2^64) mod 2^64 in
+  let v2 := (v.(Uint.value) / 2^128) mod 2^64 in
+  let v3 := (v.(Uint.value) / 2^192) mod 2^64 in
+  if (v1 =? 0) && (v2 =? 0) && (v3 =? 0) then
+    v0
+  else
+    Impl_u64.MAX.
+
+Ltac as_u64_saturated_macro_eq :=
+  unfold as_u64_saturated_macro;
+  s; [
+    apply Impl_Uint.as_limbs_eq; repeat unshelve econstructor
+  |];
+  s;
+  destruct (_ && _) in |- *; [
+    s; [
+      apply Impl_usize.max_eq
+    |];
+    s;
+    unfold M.cast_integer; cbn;
+    f_equal; [hauto lq: on | lia]
+  | s; [
+      apply Impl_u64.max_eq
+    |];
+    s; [
+      apply Impl_usize.max_eq
+    |];
+    s
+  ].
 
 Definition as_usize_saturated_macro (v : aliases.U256.t) : usize :=
-  Z.min v.(Uint.value) (2 ^ 64 - 1).
+  i[as_u64_saturated_macro v].
+
+Ltac as_usize_saturated_macro_eq :=
+  unfold as_usize_saturated_macro;
+  as_u64_saturated_macro_eq.
 
 Definition as_usize_or_fail_ret_macro {WIRE K : Set} `{Link WIRE}
     {WIRE_types : InterpreterTypes.Types.t} `{InterpreterTypes.Types.AreLinks WIRE_types}
@@ -282,54 +335,6 @@ Definition as_usize_or_fail_ret_macro {WIRE K : Set} `{Link WIRE}
         reason in
     let interpreter := interpreter <| Interpreter.control := control |> in
     k_exit interpreter.
-
-Ltac as_u64_saturated_macro_eq op1 :=
-  eapply Run.Call; [
-    apply Impl_Uint.as_limbs_eq; repeat unshelve econstructor
-  |];
-  repeat (cbn || apply Run.Pure || eapply Run.Call);
-  destruct op1 as [op1]; cbn in *;
-  assert (H_compares :
-    (
-      ((op1 / 2^64) mod 2^64 =? 0) &&
-      ((op1 / 2^128) mod 2^64 =? 0) &&
-      (op1 / 2^192 =? 0)
-    ) = true ->
-    op1 <= 2 ^ 64 - 1
-  ) by lia;
-  unfold Bool.eqb;
-  destruct (_ && _) eqn:H_and_eq; cbn;
-  [
-    eapply Run.Call; [apply Run.Pure |];
-    cbn;
-    eapply Run.Call; [apply Impl_usize.max_eq |];
-    cbn;
-    eapply Run.Call; [apply Impl_Result_T_E.unwrap_or_eq |];
-    cbn;
-    apply Run.PureEq; repeat f_equal;
-    replace (as_usize_saturated_macro _) with (op1 : usize); [
-      unfold M.cast_integer; cbn;
-      f_equal; [hauto lq: on|];
-      lia
-    |
-      unfold as_usize_saturated_macro; cbn;
-      now rewrite Z.min_l by lia
-    ]
-  |
-    eapply Run.Call; [apply Impl_u64.max_eq |];
-    cbn;
-    eapply Run.Call; [cbn; apply Run.Pure |];
-    eapply Run.Call; [apply Impl_usize.max_eq |];
-    cbn;
-    eapply Run.Call; [apply Impl_Result_T_E.unwrap_or_eq |];
-    cbn;
-    apply Run.PureEq; repeat f_equal;
-    unfold M.cast_integer, as_usize_saturated_macro; cbn;
-    f_equal; [hauto lq: on|];
-    rewrite Z.min_r; [reflexivity|];
-    assert (0 <= op1) by admit;
-    lia
-  ].
 
 Definition resize_memory_macro {WIRE K : Set} `{Link WIRE}
     {WIRE_types : InterpreterTypes.Types.t} `{InterpreterTypes.Types.AreLinks WIRE_types}
@@ -369,24 +374,3 @@ Definition resize_memory_macro {WIRE K : Set} `{Link WIRE}
   | MemoryExtensionResult.Same =>
     k interpreter
   end.
-
-Definition push_macro {WIRE K : Set} `{Link WIRE}
-    {WIRE_types : InterpreterTypes.Types.t} `{InterpreterTypes.Types.AreLinks WIRE_types}
-    {IInterpreterTypes : InterpreterTypes.C WIRE_types}
-    (interpreter : Interpreter.t WIRE WIRE_types)
-    (value : aliases.U256.t)
-    (k_exit : Interpreter.t WIRE WIRE_types -> K)
-    (k : Interpreter.t WIRE WIRE_types -> K) :
-    K :=
-  let '(success, stack) :=
-    IInterpreterTypes.(InterpreterTypes.StackTrait_for_Stack).(StackTrait.push)
-      interpreter.(Interpreter.stack) value in
-  let interpreter := interpreter <| Interpreter.stack := stack |> in
-  if success then k interpreter
-  else
-    let control :=
-      IInterpreterTypes.(InterpreterTypes.LoopControl_for_Control).(LoopControl.set_instruction_result)
-        interpreter.(Interpreter.control)
-        instruction_result.InstructionResult.StackOverflow in
-    let interpreter := interpreter <| Interpreter.control := control |> in
-    k_exit interpreter.
